EquivalenceLemmas.v
@@ -370,31 +370,3 @@ Proof.
 Qed.
 
 Hint Resolve equivalent_match_succ2: b_equiv.
-
-Lemma equivalent_tfold_congr:
-  forall t t',
-    equivalent t t' ->
-    equivalent (notype_tfold t) (notype_tfold t').
-Proof.
-  unfold equivalent in *; repeat step || t_invert_star;
-    eauto 7 using star_smallstep_trans with bsteplemmas smallstep.
-Qed.
-
-Hint Resolve equivalent_tfold_congr: b_equiv.
-
-Lemma equivalent_tunfold_congr:
-  forall t t',
-    equivalent t t' ->
-    equivalent (tunfold t) (tunfold t').
-Proof.
-  unfold equivalent in *; repeat step || t_invert_star.
-
-  - apply star_smallstep_trans with (tunfold (notype_tfold v));
-      eauto with smallstep;
-      eauto with bsteplemmas values.
-  - apply star_smallstep_trans with (tunfold (notype_tfold v));
-      eauto with smallstep;
-      eauto with bsteplemmas values.
-Qed.
-
-Hint Resolve equivalent_tunfold_congr: b_equiv.
