ReducibilityLetTermRules.v
@@ -39,6 +39,7 @@ Require Import SystemFR.RedTactics.
 Opaque reducible_values.
 Opaque makeFresh.
 
+
 Lemma reducible_value_let:
   forall theta v t A B,
     wf t 1 ->
@@ -47,7 +48,7 @@ Lemma reducible_value_let:
     valid_interpretation theta ->
     reducible_values theta v A ->
     reducible theta (open 0 t v) B ->
-    reducible theta (notype_tlet v t) B.
+    reducible theta (app (notype_lambda t) v) B.
 Proof.
   steps.
   eapply backstep_reducible; eauto using red_is_val with smallstep;
@@ -68,15 +69,16 @@ Lemma reducible_let_rule:
         is_value v ->
         star small_step t1 v ->
         reducible theta (open 0 t2 v) B) ->
-    reducible theta (notype_tlet t1 t2) B.
+    reducible theta (app (notype_lambda t2) t1) B.
 Proof.
   unfold reducible, reduces_to, closed_term; repeat step || t_listutils; eauto with bfv.
   createHypothesis;
     repeat step || t_values_info2.
   eexists; steps; eauto.
-  eapply star_smallstep_trans; eauto.
-  eapply star_smallstep_trans; eauto with bsteplemmas;
-    eauto using red_is_val with smallstep.
+  eapply star_smallstep_trans; eauto with bsteplemmas.
+  eapply star_smallstep_trans;
+    eauto with bsteplemmas values;
+    eauto with smallstep.
 Qed.
 
 Lemma open_reducible_let:
@@ -99,7 +101,7 @@ Lemma open_reducible_let:
     open_reducible tvars gamma t1 A ->
     open_reducible tvars ((p, T_equal (fvar x term_var) t1) :: (x,A) :: gamma)
                    (open 0 t2 (fvar x term_var)) B ->
-    open_reducible tvars gamma (notype_tlet t1 t2) B.
+    open_reducible tvars gamma (app (notype_lambda t2) t1) B.
 Proof.
   unfold open_reducible; steps.
 
@@ -121,7 +123,7 @@ Lemma reducible_value_let2:
     is_erased_type B ->
     reducible_values theta v A ->
     reducible theta (open 0 t v) (open 0 B v) ->
-    reducible theta (notype_tlet v t) (T_let v B).
+    reducible theta (app (notype_lambda t) v) (T_let v B).
 Proof.
   steps.
   eapply backstep_reducible; eauto using red_is_val with smallstep;
@@ -144,15 +146,17 @@ Lemma reducible_let2_rule:
         is_value v ->
         star small_step t1 v ->
         reducible theta (open 0 t2 v) (open 0 B v)) ->
-    reducible theta (notype_tlet t1 t2) (T_let t1 B).
+    reducible theta (app (notype_lambda t2) t1) (T_let t1 B).
 Proof.
   unfold reducible, reduces_to, closed_term; repeat step || t_listutils; eauto with bfv.
   createHypothesis;
     repeat step || t_values_info2.
   exists t'0; steps; eauto.
-  + eapply star_smallstep_trans; eauto.
-    eapply star_smallstep_trans; eauto with bsteplemmas;
-      eauto using red_is_val with smallstep.
+  + eapply star_smallstep_trans; eauto with bsteplemmas.
+    eapply star_smallstep_trans; eauto with bsteplemmas values.
+    eapply star_smallstep_trans;
+      eauto with bsteplemmas;
+      eauto with smallstep.
   + eapply reducible_let_backstep_values; eauto.
     eauto using reducible_val_let.
 Qed.
@@ -178,7 +182,7 @@ Lemma open_reducible_let2:
     open_reducible tvars gamma t1 A ->
     open_reducible tvars ((p, T_equal (fvar x term_var) t1) :: (x,A) :: gamma)
                    (open 0 t2 (fvar x term_var)) (open 0 B (fvar x term_var)) ->
-    open_reducible tvars gamma (notype_tlet t1 t2) (T_let t1 B).
+    open_reducible tvars gamma (app (notype_lambda t2) t1) (T_let t1 B).
 Proof.
   unfold open_reducible; steps.
 
