SwapHoles.v
@@ -76,7 +76,6 @@ Fixpoint swap_type_holes t i j :=
 
   | trefl t1 t2 => trefl (swap_type_holes t1 i j) (swap_type_holes t2 i j)
 
-  | notype_tfold t => notype_tfold (swap_type_holes t i j)
   | tfold T t => tfold (swap_type_holes T i j) (swap_type_holes t i j)
   | tunfold t => tunfold (swap_type_holes t i j)
   | tunfold_in t1 t2 => tunfold_in (swap_type_holes t1 i j) (swap_type_holes t2 i j)
